\begin{document}

\begin{equation}
\frac{D\tilde{\nu}}{Dt} = c_{b1} \tilde{S}\tilde{\nu}(1-f_{t2}) -  \Big(c_{w1}f_{w} - \frac{c_{b1}}{\kappa ^2} f_{t2} \Big) \Big(\frac{\tilde{\nu}}{d}\Big)^2 + \frac{1}{\sigma}\bigg[\frac{\partial}{\partial x_j}\Big((\nu + \tilde{\nu})\frac{\partial\tilde{\nu}}{\partial x_j}\Big) + c_{b2}\frac{\partial\tilde{\nu}}{\partial x_j}\frac{\partial\tilde{\nu}}{\partial x_j}\bigg]
\end{equation}

\begin{equation}
\frac{\partial \rho\tilde{n}}{\partial t} + \frac{\partial \rho u_j \tilde{n}}{\partial x_j} = \rho \Omega F_{crit} F_{growth}\frac{d\tilde{n}}{dRe_{\theta}} + \frac{\partial}{\partial x_j}\Big[\sigma_n(\mu + \mu_t)\frac{\partial \tilde{n}}{\partial x_j}\Big]
\end{equation}

\begin{equation}
\frac{\partial \rho \tilde{\gamma}}{\partial t} + \frac{\partial \rho u_j \tilde{\gamma}}{\partial x_j} = c_1 \rho S F_{onset} \Big[1-{{exp}} (\tilde{\gamma})\Big] - c_2 \rho \Omega F_{turb} \Big[c_3 \, {{exp}} (\tilde{\gamma}) - 1 \Big] + \frac{\partial}{\partial x_j} \bigg[\Big(\mu + \frac{\mu_t}{\sigma_y}\Big) \frac{\partial \tilde{\gamma}}{\partial x_j}\bigg]
\end{equation}

\begin{equation}
\tilde{n}
\end{equation}

\begin{equation}
H_{12}
\end{equation}

\begin{equation}
H_L = \frac{d^2}{\mu} \bigg[ \frac{\partial}{\partial x_i} \Big( \rho u_j \frac{\partial d}{\partial x_j} \Big) \frac{\partial d}{\partial x_i} \bigg]
\end{equation}

\begin{equation}
H_{12} = 0.376960 + \sqrt{\frac{H_L + 2.453432}{0.653181}}
\end{equation}

\begin{equation}
F_{crit} = 0, Re_{V} < Re_{V,0}
\end{equation}

\begin{equation}
F_{crit} = 1, Re_{V} \ge Re_{V,0}
\end{equation}

\begin{equation}
Re_{V,0} = k_V Re_{\theta,0}
\end{equation}

\begin{equation}
k_V = 0.246175{H_{12}}^2 - 0.141831 H_{12} + 0.008886
\end{equation}

\begin{equation}
Re_{V} = \frac{\rho S d^2}{\mu + \mu_t}
\end{equation}

\begin{equation}
{log}_{10} \Big(Re_{\theta ,0} \Big) = 0.7 \, {tanh} \bigg(\frac{14}{H_{12} - 1} - 9.24 \bigg) + \frac{2.492}{(H_{12} - 1)^{0.43}} + 0.62
\end{equation}

\begin{equation}
F_{growth} = D (H_{12}) \frac{1 + m(H_{12})}{2} \, l({H_{12}})
\end{equation}

\begin{equation}
D(H_{12}) = \frac{H_{12}}{0.5482 H_{12} - 0.5185}
\end{equation}

\begin{equation}
l(H_{12}) = \frac{6.54 H_{12} - 14.07}{{H_{12}}^2}
\end{equation}

\begin{equation}
m(H_{12}) = \frac{1}{l(H_{12})} \bigg[0.058 \frac{(H_{12} - 4)^2}{H_{12} - 1} - 0.068 \bigg]
\end{equation}

\begin{equation}
\frac{d \tilde{n}}{d Re_{\theta}} = 0.028 \Big( H_{12} - 1 \Big) - 0.0345 \, {exp} \bigg[- \bigg(\frac{3.87}{H_{12}-1} - 2.52 \bigg)^2 \, \bigg]
\end{equation}

\begin{equation}
\rho
\end{equation}

\begin{equation}
\mu
\end{equation}

\begin{equation}
\mu_t
\end{equation}

\begin{equation}
d
\end{equation}

\begin{equation}
S
\end{equation}

\begin{equation}
\Omega
\end{equation}

\begin{equation}
S = \sqrt{2 S_{ij} S_{ij}}
\end{equation}

\begin{equation}
S_{ij} = \frac{1}{2}\bigg(\frac{\partial u_i}{\partial x_j} + \frac{\partial u_j}{\partial x_i} \bigg)
\end{equation}

\begin{equation}
\Omega = \sqrt{2 \Omega_{ij} \Omega_{ij}}
\end{equation}

\begin{equation}
\Omega_{ij} = \frac{1}{2}\bigg(\frac{\partial u_i}{\partial x_j} - \frac{\partial u_j}{\partial x_i} \bigg)
\end{equation}

\begin{equation}
\tilde{\gamma}
\end{equation}

\begin{equation}
F_{onset} = {max} \Big[ F_{onset,2} - F_{onset,3}, 0 \Big]
\end{equation}

\begin{equation}
F_{onset,1} = \frac{\tilde{n}}{N_{crit}}
\end{equation}

\begin{equation}
F_{onset,2} = {min}\Big(F_{onset,1},2 \Big)
\end{equation}

\begin{equation}
F_{onset,3} = {max} \Big[1 - \Big(\frac{R_T}{3.5}\Big)^3, 0 \Big]
\end{equation}

\begin{equation}
F_{onset,1}
\end{equation}

\begin{equation}
F_{onset,2}
\end{equation}

\begin{equation}
F_{turb} = {exp} \bigg[ - \Big( \frac{R_T}{2} \Big)^4 \bigg]
\end{equation}

\begin{equation}
N_{crit}
\end{equation}

\begin{equation}
R_T
\end{equation}

\begin{equation}
N_{crit} = -8.43 - 2.4 {ln} \Big( {\frac{\tau}{100}} \Big)
\end{equation}

\begin{equation}
\tau =2.5 {tanh}\bigg(\frac{Tu(\%)}{2.5}\bigg)
\end{equation}

\begin{equation}
R_T = \frac{\mu_t}{\mu}
\end{equation}

\begin{equation}
Tu(\%)
\end{equation}

\begin{equation}
\tau
\end{equation}

\begin{equation}
f_{t2} = c_{t3}[1 - {exp}(\tilde{\gamma})]
\end{equation}

\begin{equation}
\sigma_n = 1.0
\end{equation}

\begin{equation}
c_1 = 100
\end{equation}

\begin{equation}
c_2 = 0.06
\end{equation}

\begin{equation}
c_3 = 50
\end{equation}

\begin{equation}
\sigma_y = 1.0
\end{equation}

\begin{equation}
c_{t3} = 1.2
\end{equation}

\begin{equation}
c_{t3}
\end{equation}

\begin{equation}
c_1
\end{equation}

\begin{equation}
c_2
\end{equation}

\begin{equation}
c_3
\end{equation}

\begin{equation}
\sigma_y
\end{equation}

\begin{equation}
\tilde{n}_{\infty} = 0
\end{equation}

\begin{equation}
\tilde{\gamma}_{\infty} = 0
\end{equation}

\begin{equation}
\frac{\partial \tilde{n}}{\partial y} \bigg|  _{wall} = 0
\end{equation}

\begin{equation}
\frac{\partial \tilde{\gamma}}{\partial y} \bigg|  _{wall} = 0
\end{equation}

\begin{equation}
2.79 {x} 10^{-7}
\end{equation}

\begin{equation}
i_t = \frac{1}{\kappa \sqrt{\nu \Omega}} \frac{\partial \tilde{\nu}}{\partial n} \bigg | _{wall}
\end{equation}

\begin{equation}
\tilde{\nu} = 0
\end{equation}

\begin{equation}
\tilde{\nu}/\nu = \kappa y^+
\end{equation}

\begin{equation}
H_L
\end{equation}

\begin{equation}
F_{growth}
\end{equation}

\begin{equation}
H_L = \frac{d^2}{\nu} \bigg[ \frac{\partial}{\partial x_i} \Big(u_j \frac{\partial d}{\partial x_j} \Big) \frac{\partial d}{\partial x_i} \bigg]
\end{equation}

\begin{equation}
H_{12} = 0.26 H_L + 2.4
\end{equation}

\begin{equation}
D(H_{12}) = \frac{2.4 H_{12}}{H_{12} - 1}
\end{equation}

\begin{equation}
k_V = \frac{1}{0.4036 {H_{12}}^2 - 2.5394 H_{12} + 4.3273}
\end{equation}

\begin{equation}
B=1
\end{equation}

\end{document}
