\begin{document}

\begin{equation}
\frac{\partial (\rho k)}{\partial t} + \frac{\partial (\rho u_j k)}{\partial x_j}
  = \cal P - \rho \epsilon  + \frac{\partial}{\partial x_j}
  \left[\left(\mu + \frac{\mu_t}{\sigma_k} \right)\frac{\partial k}{\partial x_j}\right]
  + \rho L_k
\end{equation}

\begin{equation}
\frac{\partial (\rho \epsilon)}{\partial t} + \frac{\partial (\rho u_j \epsilon)}{\partial x_j}
  = C_{\epsilon 1} f_1 \frac{\epsilon}{k} \cal P -
  C_{\epsilon 2} f_2 \frac{\rho \epsilon^2}{k} + \frac{\partial}{\partial x_j}
  \left[ \left( \mu + \frac{\mu_t}{\sigma_{\epsilon}} \right)
  \frac{\partial \epsilon}{\partial x_j} \right] +
  \rho L_{\epsilon}
\end{equation}

\begin{equation}
P = \tau_{ij} \frac{\partial u_i}{\partial x_j}
\end{equation}

\begin{equation}
\tau_{ij} = \mu_t \left(2S_{ij} - \frac{2}{3} \frac{\partial u_k}{\partial x_k} \delta_{ij} \right)
   - \frac{2}{3} \rho k \delta_{ij}
\end{equation}

\begin{equation}
S_{ij} = \frac{1}{2} \left( \frac{\partial u_i}{\partial x_j} + \frac{\partial u_j}{\partial x_i} \right)
\end{equation}

\begin{equation}
\mu_t = C_{\mu} f_{\mu} \frac{\rho k^2}{\epsilon}
\end{equation}

\begin{equation}
\rho
\end{equation}

\begin{equation}
\mu
\end{equation}

\begin{equation}
k_{wall} = 0
\end{equation}

\begin{equation}
\epsilon_{wall} = 0
\end{equation}

\begin{equation}
\sigma_k = 1.0
\end{equation}

\begin{equation}
\sigma_{\epsilon} = 1.3
\end{equation}

\begin{equation}
C_{\mu} = 0.09
\end{equation}

\begin{equation}
C_{\epsilon 1} = 1.35
\end{equation}

\begin{equation}
C_{\epsilon 2} = 1.80
\end{equation}

\begin{equation}
f_1 = 1
\end{equation}

\begin{equation}
f_2 = 1 - \frac{0.4}{1.8} e^{-Re_T^2/36}
\end{equation}

\begin{equation}
Re_T = \frac{\rho k^2}{\mu \epsilon}
\end{equation}

\begin{equation}
f_{\mu} = 1 - e^{-0.0115 d^+}
\end{equation}

\begin{equation}
d^+
\end{equation}

\begin{equation}
d^+ = d \rho u_{\tau} / \mu
\end{equation}

\begin{equation}
u_{\tau} = \sqrt{\tau_w/\rho_w}
\end{equation}

\begin{equation}
\tau_w = \mu_w \left( \frac{\partial U}{\partial n} \right)_w
\end{equation}

\begin{equation}
L_k = -2 \frac{\mu k}{\rho d^2}
\end{equation}

\begin{equation}
L_{\epsilon} = -2 \frac{\mu \epsilon}{\rho d^2} e^{-d^+/2}
\end{equation}

\begin{equation}
B=1
\end{equation}

\end{document}
