\begin{document}

\begin{equation}
\frac{\partial (\rho k)}{\partial t} + \frac{\partial (\rho u_j k)}{\partial x_j}
  = \cal P - \beta^* \rho \omega k  + \frac{\partial}{\partial x_j}
  \left[\left(\mu + \sigma_k \frac{\rho k}{\omega} \right)\frac{\partial k}{\partial x_j}\right]
\end{equation}

\begin{equation}
\frac{\partial (\rho \omega)}{\partial t} + \frac{\partial (\rho u_j \omega)}{\partial x_j}
  = \frac{\gamma \omega}{k} \cal P -
  \beta \rho \omega^2 + \frac{\partial}{\partial x_j}
  \left[ \left( \mu + \sigma_{\omega} \frac{\rho k}{\omega} \right)
  \frac{\partial \omega}{\partial x_j} \right]
\end{equation}

\begin{equation}
\mu_t = \frac{\rho k}{\omega}
\end{equation}

\begin{equation}
\sigma_k = 0.5
\end{equation}

\begin{equation}
\sigma_{\omega} = 0.5
\end{equation}

\begin{equation}
\beta^* = 0.09
\end{equation}

\begin{equation}
\beta = \frac{3}{40}
\end{equation}

\begin{equation}
\gamma = \frac{5}{9}
\end{equation}

\begin{equation}
\gamma
\end{equation}

\begin{equation}
\alpha
\end{equation}

\begin{equation}
\kappa \approx 0.408
\end{equation}

\begin{equation}
\gamma = \frac{\beta}{\beta^*} - \frac{\sigma_{\omega} \kappa^2}{\sqrt{\beta^*}}
\end{equation}

\begin{equation}
B=1
\end{equation}

\end{document}
