\begin{document}

\begin{equation}
c_{b1} \hat S \hat \nu
\end{equation}

\begin{equation}
f_{r1}
\end{equation}

\begin{equation}
f_{r1} = (1 + c_{r1}) \frac{2r^*}{1+r^*}\left[ 1 - c_{r3} {\rm tan}^{-1}(c_{r2} \hat r)\right] - c_{r1}
\end{equation}

\begin{equation}
r^* = S/\omega
\end{equation}

\begin{equation}
\hat r = \frac{2 \omega_{ik} S_{jk}}{D^4} \left( \frac{DS_{ij}}{Dt} + (\varepsilon_{imn}S_{jn}
   +\varepsilon_{jmn}S_{in}) \Omega'_m \right)
\end{equation}

\begin{equation}
S_{ij} = \frac{1}{2} \left(\frac{\partial u_i}{\partial x_j} + 
   \frac{\partial u_j}{\partial x_i} \right)
\end{equation}

\begin{equation}
\omega_{ij} = \frac{1}{2} \left[ \left(\frac{\partial u_i}{\partial x_j} - 
   \frac{\partial u_j}{\partial x_i} \right) + 2 \varepsilon_{mji} \Omega'_m \right]
\end{equation}

\begin{equation}
S^2 = 2 S_{ij}S_{ij}
\end{equation}

\begin{equation}
\omega^2 = 2 \omega_{ij}\omega_{ij}
\end{equation}

\begin{equation}
D^2 = \frac{1}{2} \left(S^2 + \omega^2 \right)
\end{equation}

\begin{equation}
c_{r1} = 1.0
\end{equation}

\begin{equation}
c_{r2} = 12
\end{equation}

\begin{equation}
c_{r3} = 1.0
\end{equation}

\begin{equation}
DS_{ij}/Dt
\end{equation}

\begin{equation}
\Omega'
\end{equation}

\begin{equation}
\frac{D S_{ij}}{Dt} \equiv \frac{\partial S_{ij}}{\partial t} +
   u_k \frac{\partial S_{ij}}{\partial x_k}
\end{equation}

\begin{equation}
c_{b1}(f_{r1}-f_{t2})\hat S \hat \nu
\end{equation}

\begin{equation}
B=1
\end{equation}

\end{document}
