\begin{document}

\begin{equation}
Re_{\theta} = \frac{\rho_{\infty} U_{\infty} \theta}{\mu_{\infty}}
\end{equation}

\begin{equation}
\theta = \int_0^{\infty} \frac{\rho}{\rho_{\infty}} \frac{u}{U_{\infty}} \left( 1 - \frac{u}{U_{\infty}} \right) dy
\end{equation}

\begin{equation}
c_f = \frac{\tau_w}{\frac{1}{2} \rho_{\infty} U_{\infty}^2}
\end{equation}

\begin{equation}
\tau_w = \mu_w \left( \frac{\partial u}{\partial y} \right)_w
\end{equation}

\begin{equation}
u^+ = \frac{u}{v^*} = \frac{u}{\sqrt{\tau_w / \rho_w}}
\end{equation}

\begin{equation}
y^+ = \frac{y v^*}{\nu_w} = \frac{y \sqrt{\tau_w / \rho_w}}{\nu_w}
\end{equation}

\begin{equation}
c_{f,incomp}(Re_{\theta}) = \left( 17.08 \left({\rm log}_{10}Re_{\theta} \right)^2 + 25.11 \left( {\rm log}_{10}Re_{\theta} \right) +
   6.012 \right)^{-1}
\end{equation}

\begin{equation}
u^+_{incomp} = \frac{1}{\kappa} {\rm ln} \left( y^+ \right) + C + \frac{2 \Pi}{\kappa}
\left[ {\rm sin} \left( \frac{\pi y}{2 \delta} \right) \right]^2
\end{equation}

\begin{equation}
T_{aw}=T_{\infty}\left(1+r\frac{\gamma-1}{2}M^2 \right)
\end{equation}

\begin{equation}
C_f = \frac{1}{F_c} {c_{f,incomp}} \left(Re_{\theta}^{'}\right)
\end{equation}

\begin{equation}
F_{Re\theta}=\frac{\mu_\infty}{\mu_w}
\end{equation}

\begin{equation}
F_{Re\theta}={\left(\frac{T_\infty}{T_w}}\right)^{3/2}\frac{T_w+110.4}{T_\infty+110.4}
\end{equation}

\begin{equation}
F_c=\frac{T_{aw}/T_\infty-1}{\left(sin^{-1}A+sin^{-1}B)\right^2}
\end{equation}

\begin{equation}
A=\frac{2a^{2}-b}{\left(b^{2}+4a^{2})\right^{1/2}
\end{equation}

\begin{equation}
B=\frac{b}{\left(b^{2}+4a^{2})\right^{1/2}
\end{equation}

\begin{equation}
a=\left(r\frac{\gamma-1}{2}M^{2}\frac{T_\infty}{T_w}\right)^{1/2}=\left[\left(\frac{T_{aw}}{T_\infty}-1\right)\frac{T_\infty}{T_w}\right]^{1/2}
\end{equation}

\begin{equation}
b=\frac{T_{aw}}{T_w}-1
\end{equation}

\begin{equation}
u_{eqiv}^{+}=\frac{u_{eqiv}}{u_\tau}=\frac{1}{\kappa} {\rm ln} \left( y^+ \right) + C + \frac{2 \Pi}{\kappa}
\left[ {\rm sin} \left( \frac{\pi y}{2 \delta} \right) \right]^2
\end{equation}

\begin{equation}
Q=\left(b^{2}+4a^{2}\right)^{1/2}
\end{equation}

\begin{equation}
u_{eqiv}^{+}=\frac{u_{eqiv}}{u_\tau}=\frac{u_\infty}{au_\tau}\left(sin^{-1}\frac{2a^{2}\frac{u}{u_\infty}-b}{Q}+sin^{-1}\frac{b}{Q}\right)
\end{equation}

\begin{equation}
u^{+}=\frac{u}{u_\tau}=\frac{u_\infty}{2u_{\tau}a^2}\left[Q*sin\left(\frac{au_\tau}{u_\infty}u_{incomp}^{+}-sin^{-1}\frac{b}{Q}\right)+b\right]
\end{equation}

\begin{equation}
u_\tau=\sqrt{\frac{\tau_w}{\rho_w}}
\end{equation}

\begin{equation}
\tau_w=\frac{1}{2}\rho_{\infty}u_{\infty}^{2}c_f
\end{equation}

\begin{equation}
\rho_\infty=\frac{p_\infty}{R_{gas}T_\infty}
\end{equation}

\begin{equation}
\rho_w=\frac{p_\infty}{R_{gas}T_w}
\end{equation}

\begin{equation}
u_\infty=\sqrt{{\gamma}R_{gas}T_\infty}M_\infty
\end{equation}

\begin{equation}
{Re}_{\theta}^{'}=Re_{\theta}F_{Re\theta}
\end{equation}

\begin{equation}
B=1
\end{equation}

\end{document}
