\begin{document}

\begin{equation}
\tau_{ij} = 2 \mu_t \left(S_{ij} - \frac{1}{3} \frac{\partial u_k}{\partial x_k} \delta_{ij} \right) -
  \frac{2}{3} \rho k \delta_{ij}
\end{equation}

\begin{equation}
(2/3) \rho k \delta_{ij}
\end{equation}

\begin{equation}
\mu_t
\end{equation}

\begin{equation}
\tau_{ij}
\end{equation}

\begin{equation}
\tau_{ij} = 2 \mu_t \left(S_{ij} - \frac{1}{3} \frac{\partial u_k}{\partial x_k} \delta_{ij} 
  + \left[a_2 a_4 \left( S_{ik}W_{kj} - W_{ik}S_{kj}\right) - 2 a_3 a_4 \left(S_{ik}S_{kj} - \frac{1}{3}S_{kl}S_{lk}\delta_{ij}\right)
  \right] \right) -
  \frac{2}{3} \rho k \delta_{ij}
\end{equation}

\begin{equation}
\frac{\partial (\rho k)}{\partial t} + \frac{\partial (\rho u_j k)}{\partial x_j}
  = \cal P - f_{\beta^*} \rho \omega k  + \frac{\partial}{\partial x_j}
\left[\left(\mu + \sigma_k \mu_t \right)\frac{\partial k}{\partial x_j}\right]
\end{equation}

\begin{equation}
\frac{\partial (\rho \omega)}{\partial t} + \frac{\partial (\rho u_j \omega)}{\partial x_j}
  = \frac{\gamma \omega}{k} \cal P -
  \beta \rho \omega^2 + \frac{\partial}{\partial x_j}
  \left[ \left( \mu + \sigma_{\omega} \mu_t \right)
  \frac{\partial \omega}{\partial x_j} \right]
\end{equation}

\begin{equation}
P = \tau_{ij} \frac{\partial u_i}{\partial x_j}
\end{equation}

\begin{equation}
S_{ij} = \frac{1}{2} \left( \frac{\partial u_i}{\partial x_j} + \frac{\partial u_j}{\partial x_i} \right)
\end{equation}

\begin{equation}
W_{ij} = \frac{1}{2} \left( \frac{\partial u_i}{\partial x_j} - \frac{\partial u_j}{\partial x_i} \right)
\end{equation}

\begin{equation}
\mu_t = C_{\mu}^* \frac{\rho k}{\omega}
\end{equation}

\begin{equation}
\rho
\end{equation}

\begin{equation}
\mu
\end{equation}

\begin{equation}
C_{\mu}^*
\end{equation}

\begin{equation}
(-C_{\mu}^*)^3 + p(-C_{\mu}^*)^2 + q(-C_{\mu}^*) + r = 0
\end{equation}

\begin{equation}
p = - \frac{\gamma_1^*}{\eta^2 \tau^2 \gamma_0^*}
\end{equation}

\begin{equation}
q = \frac{1}{(2 \eta^2 \tau^2 \gamma_0^*)^2} \left( \gamma_1^{*2} - 2 \eta^2 \tau^2 \gamma_0^* a_1
  -\frac{2}{3} \eta^2 \tau^2 a_3^2 + 2 R^2 \eta^2 \tau^2 a_2^2 \right)
\end{equation}

\begin{equation}
r = \frac{\gamma_1^* a_1}{(2 \eta^2 \tau^2 \gamma_0^*)^2}
\end{equation}

\begin{equation}
\eta \rightarrow 0
\end{equation}

\begin{equation}
\tau \equiv 1 / \omega
\end{equation}

\begin{equation}
\eta^2 = \lbrace S^2 \rbrace = S_{ij}S_{ij}
\end{equation}

\begin{equation}
\lbrace W^2 \rbrace = -W_{ij}W_{ij}
\end{equation}

\begin{equation}
R^2 = - \frac{\lbrace W^2 \rbrace}{\lbrace S^2 \rbrace}
\end{equation}

\begin{equation}
a_1 = \frac{1}{2} \left( \frac{4}{3} - C_2 \right)
\end{equation}

\begin{equation}
a_2 = \frac{1}{2} \left( 2 - C_4 \right)
\end{equation}

\begin{equation}
a_3 = \frac{1}{2} \left( 2 - C_3 \right)
\end{equation}

\begin{equation}
a_4 = \tau \left[ \gamma_1^* - 2 \gamma_0^* \left( -C_{\mu}^* \right) \eta^2 \tau^2 \right]^{-1}
\end{equation}

\begin{equation}
\gamma_0^* = \frac{C_1^1}{2}
\end{equation}

\begin{equation}
\gamma_1^* = \frac{1}{2} C_1^0 + \left( \frac{C_{\epsilon 2} - C_{\epsilon 1}}{C_{\epsilon 1} - 1} \right)
\end{equation}

\begin{equation}
f_{\beta^*}
\end{equation}

\begin{equation}
f_{\beta^*} = 1 
\end{equation}

\begin{equation}
\chi_k \leq 0
\end{equation}

\begin{equation}
f_{\beta^*} = \frac{1 + 680 \chi_k^2}{1 + 400 \chi_k^2}
\end{equation}

\begin{equation}
\chi_k > 0
\end{equation}

\begin{equation}
\chi_k = \frac{C_{\mu}^2}{\omega^3} \frac{\partial k}{\partial x_j} \frac{\partial \omega}{\partial x_j}
\end{equation}

\begin{equation}
{\rm min}(P, 20 f_{\beta^*} \rho \omega k)
\end{equation}

\begin{equation}
\tau_{11}
\end{equation}

\begin{equation}
\tau_{22}
\end{equation}

\begin{equation}
\tau_{33}
\end{equation}

\begin{equation}
\overline k_{farfield} = \frac{k_{farfield}}{a_{ref}^2} = 9 \times 10^{-9}
\end{equation}

\begin{equation}
\overline \omega_{farfield} = \frac{\omega_{farfield}}{(\rho_{ref} a_{ref}^2/ \mu_{ref} )} = 9 \times 10^{-8}
\end{equation}

\begin{equation}
\rho_{ref}
\end{equation}

\begin{equation}
a_{ref}
\end{equation}

\begin{equation}
\mu_{ref}
\end{equation}

\begin{equation}
\omega_{wall} = 10 \frac{6 \nu}{\beta (\Delta d_1)^2}
\end{equation}

\begin{equation}
k_{wall} = 0
\end{equation}

\begin{equation}
\Delta d_1
\end{equation}

\begin{equation}
C_{\epsilon 1} = 1.44
\end{equation}

\begin{equation}
C_{\epsilon 2} = 1.83
\end{equation}

\begin{equation}
C_1^0 = 3.4
\end{equation}

\begin{equation}
C_1^1 = 1.8
\end{equation}

\begin{equation}
C_2 = 0.36
\end{equation}

\begin{equation}
C_3 = 1.25
\end{equation}

\begin{equation}
C_4 = 0.4
\end{equation}

\begin{equation}
C_{\mu} = 0.0895
\end{equation}

\begin{equation}
\sigma_k = 1
\end{equation}

\begin{equation}
\sigma_{\omega} = \sqrt{C_{\mu}}(\beta - \gamma)/(\kappa^2)
\end{equation}

\begin{equation}
\kappa = 0.41
\end{equation}

\begin{equation}
\gamma = 0.53
\end{equation}

\begin{equation}
\beta = 0.83
\end{equation}

\begin{equation}
P = 2 \mu_t \eta^2 = 2 \mu_t S_{ij} S_{ij}
\end{equation}

\begin{equation}
\sigma_k = 0.5
\end{equation}

\begin{equation}
\gamma = 0.575
\end{equation}

\begin{equation}
\eta^2 \tau^2 < 1 \times 10^{-6}
\end{equation}

\begin{equation}
C_{\mu}^* = \frac{\gamma_1^* a_1}{\gamma_1^{*2} - 2 \lbrace W^2 \rbrace \tau^2 a_2^2}
\end{equation}

\begin{equation}
a \equiv q - \frac{p^2}{3}
\end{equation}

\begin{equation}
b \equiv \frac{1}{27} \left( 2 p^3 - 9 p q + 27 r \right)
\end{equation}

\begin{equation}
d \equiv \frac{b^2}{4} + \frac{a^3}{27}
\end{equation}

\begin{equation}
d > 0
\end{equation}

\begin{equation}
t_1 = \left( -\frac{b}{2} + \sqrt{d} \right)^{1/3}
\end{equation}

\begin{equation}
t_2 = \left( -\frac{b}{2} - \sqrt{d} \right)^{1/3}
\end{equation}

\begin{equation}
C_{\mu}^* = -{\rm min} \left( -\frac{p}{3} + t_1 + t_2, -\frac{p}{3} -\frac{t_1}{2} - \frac{t_2}{2} \right)
\end{equation}

\begin{equation}
d \leq 0
\end{equation}

\begin{equation}
\theta = {\rm cos}^{-1} \left( - \frac{b/2}{\sqrt{-a^3/27} \right)
\end{equation}

\begin{equation}
t_1 = -\frac{p}{3} + 2 \sqrt{-\frac{a}{3} } {\rm cos} \left( \frac{\theta}{3} \right)
\end{equation}

\begin{equation}
t_2 = -\frac{p}{3} + 2 \sqrt{-\frac{a}{3} } {\rm cos} \left( \frac{2 \pi}{3} + \frac{\theta}{3} \right)
\end{equation}

\begin{equation}
t_3 = -\frac{p}{3} + 2 \sqrt{-\frac{a}{3} } {\rm cos} \left( \frac{4 \pi}{3} + \frac{\theta}{3} \right)
\end{equation}

\begin{equation}
C_{\mu}^* = -{\rm min} \left( t_1 , t_2 , t_3 \right)
\end{equation}

\begin{equation}
B=1
\end{equation}

\end{document}
