\begin{document}

\begin{equation}
\mu = \mu_0 \left( \frac{T}{T_0} \right)^{3/2} \left(
\frac{T_0 + S}{T+S} \right)
\end{equation}

\begin{equation}
\mu_0 = 1.716 \times 10^{-5} kg/(ms)
\end{equation}

\begin{equation}
T_0 = 491.6 R
\end{equation}

\begin{equation}
S = 198.6 R
\end{equation}

\begin{equation}
\left( \frac{\mu}{\mu_{ref}} \right) = \left( \frac{T}{T_{ref}} \right)^{3/2} \left(
\frac{T_{ref} + S}{T+S} \right)
\end{equation}

\begin{equation}
\mu_{ref}
\end{equation}

\begin{equation}
T_{ref}
\end{equation}

\begin{equation}
B=1
\end{equation}

\end{document}
