\begin{document}

\begin{equation}
\frac{\partial (\rho k)}{\partial t} + \frac{\partial (\rho u_j k)}{\partial x_j}
  = \cal P - \beta^* \rho \omega k  + \frac{\partial}{\partial x_j}
  \left[\left(\mu + \sigma_k \frac{\rho k}{\omega} \right)\frac{\partial k}{\partial x_j}\right]
\end{equation}

\begin{equation}
\frac{\partial (\rho \omega)}{\partial t} + \frac{\partial (\rho u_j \omega)}{\partial x_j}
  = \frac{\gamma \omega}{k} \cal P -
  \beta \rho \omega^2 + \frac{\partial}{\partial x_j}
  \left[ \left( \mu + \sigma_{\omega} \frac{\rho k}{\omega} \right)
  \frac{\partial \omega}{\partial x_j} \right]
\end{equation}

\begin{equation}
\mu_t = \frac{\rho k}{\omega}
\end{equation}

\begin{equation}
\sigma_k = 0.5
\end{equation}

\begin{equation}
\sigma_{\omega} = 0.5
\end{equation}

\begin{equation}
\beta_0^* = 0.09
\end{equation}

\begin{equation}
\gamma = \frac{13}{25}
\end{equation}

\begin{equation}
\beta = \beta_0 f_{\beta}
\end{equation}

\begin{equation}
\beta_0 = \frac{9}{125}
\end{equation}

\begin{equation}
f_{\beta} = \frac{1 + 70 \chi_{\omega}}{1 + 80 \chi_{\omega}}
\end{equation}

\begin{equation}
\chi_{\omega} = \left| \frac{\Omega_{ij} \Omega_{jk} S_{ki}}
  {(\beta_0^* \omega)^3} \right|
\end{equation}

\begin{equation}
\beta^* = \beta_0^* f_{\beta^*}
\end{equation}

\begin{equation}
f_{\beta^*} = 1, \quad for \quad \left( \chi_k \leq 0 \right)
\end{equation}

\begin{equation}
f_{\beta^*} = \frac{1+680 \chi_k^2}{1+400 \chi_k^2}, \quad for \quad \left( 
  \chi_k > 0 \right)
\end{equation}

\begin{equation}
\chi_k = \frac{1}{\omega^3} \frac{\partial k}{\partial x_j}
  \frac{\partial \omega}{\partial x_j}
\end{equation}

\begin{equation}
\gamma
\end{equation}

\begin{equation}
\alpha
\end{equation}

\begin{equation}
\kappa \approx 0.41
\end{equation}

\begin{equation}
\gamma = \frac{\beta_0}{\beta_0^*} - \frac{\sigma_{\omega} \kappa^2}{\sqrt{\beta_0^*}}
\end{equation}

\begin{equation}
B=1
\end{equation}

\end{document}
