\begin{document}

\begin{equation}
\beta^* = 0.09
\end{equation}

\begin{equation}
\beta^* = 0.09 \left( \frac{100 \beta_0 / 27 + (Re_T/R_{\beta})^4}
{1 + (Re_T/R_{\beta})^4} \right)
\end{equation}

\begin{equation}
\gamma = 13/25
\end{equation}

\begin{equation}
\gamma = 13/25 \left( \frac{\alpha_0 + Re_T/R_{\omega}}
{1 + Re_T/R_{\omega}} \right) (\alpha^*)^{-1}
\end{equation}

\begin{equation}
\mu_t = \rho k / \hat\omega
\end{equation}

\begin{equation}
\mu_t = \alpha^* \frac{\rho k}{\hat\omega}
\end{equation}

\begin{equation}
\hat\omega = {\rm max} (\omega, C_{lim} \sqrt{2 \overline S_{ij} \overline S_{ij} / \beta^*} )
\end{equation}

\begin{equation}
\hat\omega = {\rm max} \left(\omega, C_{lim} \sqrt{ \frac{2 \overline S_{ij} \overline S_{ij}}{\beta_0^*/\alpha^*}} \right)
\end{equation}

\begin{equation}
(\mu + \sigma_k (\rho k / \omega))
\end{equation}

\begin{equation}
k
\end{equation}

\begin{equation}
\left(\mu + \sigma_k \alpha^* \frac{\rho k}{\omega} \right)
\end{equation}

\begin{equation}
(\mu + \sigma_{\omega} (\rho k / \omega))
\end{equation}

\begin{equation}
\omega
\end{equation}

\begin{equation}
\left(\mu + \sigma_{\omega} \alpha^* \frac{\rho k}{\omega} \right)
\end{equation}

\begin{equation}
Re_T = \frac{\rho k}{\mu \omega}
\end{equation}

\begin{equation}
\alpha^* = \frac{\alpha_0^* + Re_T/R_k}{1 + Re_T/R_k}
\end{equation}

\begin{equation}
R_{\beta} = 8
\end{equation}

\begin{equation}
R_k = 6
\end{equation}

\begin{equation}
R_{\omega} = 2.61
\end{equation}

\begin{equation}
\alpha_0 = \frac{1}{9}
\end{equation}

\begin{equation}
\alpha_0^* = \frac{\beta_0}{3}
\end{equation}

\begin{equation}
\beta_0 = 0.0708
\end{equation}

\begin{equation}
\beta_0^* = 0.09
\end{equation}

\begin{equation}
B=1
\end{equation}

\end{document}
