\begin{document}

\begin{equation}
\tau_{ij}
\end{equation}

\begin{equation}
\overline \rho \hat R_{ij}
\end{equation}

\begin{equation}
-\tau_{ij}
\end{equation}

\begin{equation}
\overline \rho \hat R_{ij} = -\tau_{ij} = \overline {\rho u_i'' u_j''}
\end{equation}

\begin{equation}
\frac{\partial \overline \rho \hat R_{ij}}{\partial t} +
\frac{\partial (\overline \rho \hat u_k \hat R_{ij})}{\partial x_k} = \overline \rho P_{ij} +
\overline \rho \Pi_{ij} - \overline \rho \varepsilon_{ij} + \overline \rho D_{ij} +
\overline \rho M_{ij}
\end{equation}

\begin{equation}
\overline \rho P_{ij} = - \overline \rho \hat R_{ik}
\frac{\partial \hat u_j}{\partial x_k}
- \overline \rho \hat R_{jk}
\frac{\partial \hat u_i}{\partial x_k}
\end{equation}

\begin{equation}
\overline \rho \varepsilon_{ij} = \frac{2}{3} \overline \rho \varepsilon \delta_{ij}
\end{equation}

\begin{equation}
\varepsilon = C_{\mu} \hat k \omega
\end{equation}

\begin{equation}
\hat k = \hat R_{ii}/2
\end{equation}

\begin{equation}
\overline \rho \Pi_{ij} = - \left( C_1 \overline \rho \varepsilon +
\frac{1}{2} C_1^* \overline \rho P_{kk} \right) \hat a_{ij} +
C_2 \overline \rho \varepsilon \left( \hat a_{ik} \hat a_{kj} -
\frac{1}{3} \hat a_{kl} \hat a_{kl} \delta_{ij} \right) +
\left( C_3 - C_3^* \sqrt{\hat a_{kl} \hat a_{kl}} \right)
\overline \rho \hat k \hat S_{ij}^* +
C_4 \overline \rho \hat k \left( \hat a_{ik} \hat S_{jk} +
\hat a_{jk} \hat S_{ik} - \frac{2}{3} \hat a_{kl} \hat S_{kl} \delta_{ij} \right) +
C_5 \overline \rho \hat k \left( \hat a_{ik} \hat W_{jk} + \hat a_{jk} \hat W_{ik} \right)
\end{equation}

\begin{equation}
\hat a_{ij} = \frac{\hat R_{ij}}{\hat k} - \frac{2}{3} \delta_{ij}
\end{equation}

\begin{equation}
\hat S_{ij} = \frac{1}{2} \left( \frac{\partial \hat u_i}{\partial x_j} +
\frac{\partial \hat u_j}{\partial x_i} \right)
\end{equation}

\begin{equation}
\hat S_{ij}^* = \hat S_{ij} - \frac{1}{3} \hat S_{kk} \delta_{ij}
\end{equation}

\begin{equation}
\hat W_{ij} = \frac{1}{2} \left( \frac{\partial \hat u_i}{\partial x_j} -
\frac{\partial \hat u_j}{\partial x_i} \right)
\end{equation}

\begin{equation}
\overline \rho D_{ij} = \frac{\partial}{\partial x_k}
\left[ \left( \overline \mu \delta_{kl} + D \frac{\overline \rho \hat k \hat R_{kl}}{\varepsilon}
\right) \frac{\partial \hat R_{ij}}{\partial x_l} \right]
= \frac{\partial}{\partial x_k}
\left[ \left( \overline \mu \delta_{kl} + D \frac{\overline \rho \hat R_{kl}}{C_{\mu} \omega}
\right) \frac{\partial \hat R_{ij}}{\partial x_l} \right]
\end{equation}

\begin{equation}
\overline \rho M_{ij}
\end{equation}

\begin{equation}
\frac{\partial (\overline \rho \omega)}{\partial t} +
  \frac{\partial (\overline \rho \hat u_k \omega)}{\partial x_k}
  = \frac{\alpha_{\omega} \omega}{\hat k} \frac{\overline \rho P_{kk}}{2} -
  \beta_{\omega} \overline \rho \omega^2 + \frac{\partial}{\partial x_k}
  \left[ \left( \overline \mu + \sigma_{\omega} \frac{\overline \rho \hat k}{\omega} \right)
  \frac{\partial \omega}{\partial x_k} \right] +
  \sigma_d \frac{\overline \rho}{\omega} {\rm max} \left( \frac{\partial \hat k}{\partial x_j}
  \frac{\partial \omega}{\partial x_j}, 0 \right)
\end{equation}

\begin{equation}
\phi = F_1 \phi^{(\omega)} + (1-F_1) \phi^{(\varepsilon)}
\end{equation}

\begin{equation}
F_1 = tanh(\zeta^4)
\end{equation}

\begin{equation}
\zeta = {\rm min} \left[ {\rm max} \left(
\frac{\sqrt{\hat k}}{C_{\mu} \omega d} , \frac{500 \hat \mu}{\overline \rho \omega d^2} \right) ,
\frac{4 \sigma_{\omega}^{(\varepsilon)}\overline \rho \hat k}
{(CD) d^2} \right]
\end{equation}

\begin{equation}
(CD) = \sigma_d^{(\varepsilon)} \frac{\overline \rho}{\omega}
{\rm max} \left( \frac{\partial \hat k}{\partial x_k}
\frac{\partial \omega}{\partial x_k}, 0 \right)
\end{equation}

\begin{equation}
C_{\mu} = 0.09
\end{equation}

\begin{equation}
\omega
\end{equation}

\begin{equation}
\alpha_{\omega}^{(\omega)} = 0.5556
\end{equation}

\begin{equation}
\beta_{\omega}^{(\omega)} = 0.075
\end{equation}

\begin{equation}
\sigma_{\omega}^{(\omega)} = 0.5
\end{equation}

\begin{equation}
\sigma_d^{(\omega)} = 0
\end{equation}

\begin{equation}
C_1^{(\omega)} = 1.8
\end{equation}

\begin{equation}
C_1^{*(\omega)} = 0
\end{equation}

\begin{equation}
C_2^{(\omega)} = 0
\end{equation}

\begin{equation}
C_3^{(\omega)} = 0.8
\end{equation}

\begin{equation}
C_3^{*(\omega)} = 0
\end{equation}

\begin{equation}
C_4^{(\omega)} = 0.5 (18 C_2^{(LRR)} + 12) / 11
\end{equation}

\begin{equation}
C_5^{(\omega)} = 0.5 (-14 C_2^{(LRR)} + 20)/11
\end{equation}

\begin{equation}
D^{(\omega)} = 0.75 C_{\mu}
\end{equation}

\begin{equation}
\varepsilon
\end{equation}

\begin{equation}
\alpha_{\omega}^{(\varepsilon)} = 0.44
\end{equation}

\begin{equation}
\beta_{\omega}^{(\varepsilon)} = 0.0828
\end{equation}

\begin{equation}
\sigma_{\omega}^{(\varepsilon)} = 0.856
\end{equation}

\begin{equation}
\sigma_d^{(\varepsilon)} = 1.712
\end{equation}

\begin{equation}
C_1^{(\varepsilon)} = 1.7
\end{equation}

\begin{equation}
C_1^{*(\varepsilon)} = 0.9
\end{equation}

\begin{equation}
C_2^{(\varepsilon)} = 1.05
\end{equation}

\begin{equation}
C_3^{(\varepsilon)} = 0.8
\end{equation}

\begin{equation}
C_3^{*(\varepsilon)} = 0.65
\end{equation}

\begin{equation}
C_4^{(\varepsilon)} = 0.625
\end{equation}

\begin{equation}
C_5^{(\varepsilon)} = 0.2
\end{equation}

\begin{equation}
D^{(\varepsilon)} = 0.22
\end{equation}

\begin{equation}
c_p \overline {\rho u_j'' T''} \approx
-\frac{c_p \mu_t}{Pr_t} \frac{\partial \hat T}{\partial x_j}
\end{equation}

\begin{equation}
\mu_t
\end{equation}

\begin{equation}
\mu_t=\overline \rho \hat k / \omega
\end{equation}

\begin{equation}
\frac{\partial}{\partial x_k} \left(
\overline{\sigma_{ij} u_i''} - \frac{1}{2} \overline{\rho u_i'' u_i'' u_j''} \right) \approx
\frac{1}{2} \left( \overline \rho T_{ii} + \overline \rho D_{ii}^{(\nu)} \right)
\end{equation}

\begin{equation}
\overline \rho T_{ij} = \frac{\partial}{\partial x_k} \left(
D \frac{\overline \rho \hat k \hat R_{kl}}{\varepsilon}
\frac{\partial \hat R_{ij}}{\partial x_l} \right)
\end{equation}

\begin{equation}
\overline \rho D_{ij}^{(\nu)} = \frac{\partial}{\partial x_k} \left(
\overline \mu \frac{\partial \hat R_{ij}}{\partial x_k} \right)
\end{equation}

\begin{equation}
\hat R_{ij, farfield} = \frac{2}{3} \hat k_{farfield} \delta_{ij}
\end{equation}

\begin{equation}
\omega_{farfield} = \frac{\overline \rho \hat k_{farfield}}{\mu_{t, farfield}}
\end{equation}

\begin{equation}
\hat k_{farfield}
\end{equation}

\begin{equation}
\mu_{t, farfield}
\end{equation}

\begin{equation}
\hat k_{farfield} = (3/2) (Tu)^2 U_{farfield}^2
\end{equation}

\begin{equation}
\mu_{t, farfield}/\overline \mu_{farfield} = 0.1
\end{equation}

\begin{equation}
\hat R_{ij, wall} = 0
\end{equation}

\begin{equation}
\omega_{wall} = 10 \frac{6 \hat \nu}{\beta_{\omega}^{(\omega)} (\Delta d_1)^2}
\end{equation}

\begin{equation}
\Delta d_1
\end{equation}

\begin{equation}
C_2^{(LRR)}
\end{equation}

\begin{equation}
D^{(\omega)}
\end{equation}

\begin{equation}
C_2^{(LRR)} = 0.52
\end{equation}

\begin{equation}
C_4^{(\omega)}
\end{equation}

\begin{equation}
C_5^{(\omega)}
\end{equation}

\begin{equation}
\overline \rho D_{ij}
\end{equation}

\begin{equation}
\overline \rho D_{ij} = \frac{\partial}{\partial x_k}
\left[ \left( \overline \mu + D \frac{\overline \rho \hat k^2}{\varepsilon}
\right) \frac{\partial \hat R_{ij}}{\partial x_k} \right]
= \frac{\partial}{\partial x_k}
\left[ \left( \overline \mu + D \frac{\overline \rho \hat k}{C_{\mu} \omega}
\right) \frac{\partial \hat R_{ij}}{\partial x_k} \right]
= \frac{\partial}{\partial x_k}
\left[ \left( \overline \mu + \frac{D}{C_{\mu}} \mu_t
\right) \frac{\partial \hat R_{ij}}{\partial x_k} \right]
\end{equation}

\begin{equation}
D = 0.5 C_{\mu} F_1 + \frac{2}{3} 0.22 (1-F_1)
\end{equation}

\begin{equation}
\overline {\rho u_i'' u_i''} \geq 0
\end{equation}

\begin{equation}
i \in {1,2,3}
\end{equation}

\begin{equation}
\left|\overline {\rho u_i'' u_j''}\right| \leq 
\sqrt{\left(\overline {\rho u_i'' u_i''}\right) \left(\overline {\rho u_j'' u_j''}\right)}
\end{equation}

\begin{equation}
i,j \in {1,2,3}
\end{equation}

\begin{equation}
{\rm det}\left(\overline {\rho u_i'' u_j''}\right) \geq 0
\end{equation}

\begin{equation}
B=1
\end{equation}

\end{document}
