\begin{document}

\begin{equation}
\overline{u'v'}
\end{equation}

\begin{equation}
\tau_{ij} \equiv - \overline{\rho u_i''u_j''}
\end{equation}

\begin{equation}
\overline{\rho u_i''u_j''}
\end{equation}

\begin{equation}
\overline{\rho} \overline{u_i'u_j'}
\end{equation}

\begin{equation}
\overline{u_i'u_j'} \approx - \frac{\tau_{ij}}{\overline{\rho}}
\end{equation}

\begin{equation}
\tau_{ij}
\end{equation}

\begin{equation}
\overline{u'v'} = - \frac{\hat \mu_t}{\overline{\rho}} \left(
\frac{\partial \hat u}{\partial y} + \frac{\partial \hat v}{\partial x} \right)
\end{equation}

\begin{equation}
C_f = \frac{2 \tau_w}{\rho_{ref}U_{ref}^2}
\end{equation}

\begin{equation}
\tau_w
\end{equation}

\begin{equation}
\tau_w=\mu_w \left( \frac{\partial u'}{\partial n} \right)_w 
\end{equation}

\begin{equation}
\mu
\end{equation}

\begin{equation}
C_p = \frac{2 \left(p_w-p_{ref}\right)}{\rho_{ref}U_{ref}^2}
\end{equation}

\begin{equation}
C_L = \frac{2 L}{\rho_{ref}U_{ref}^2 A}
\end{equation}

\begin{equation}
C_D = \frac{2 D}{\rho_{ref}U_{ref}^2 A}
\end{equation}

\begin{equation}
B=1
\end{equation}

\end{document}
