\begin{document}

\begin{equation}
\frac{\partial \rho k}{\partial t} +
\frac{\partial (\rho u_j k)}{\partial x_j} = P - \rho \varepsilon +
\frac{\partial}{\partial x_j} \left[
\left( \mu + \frac{\mu_t}{\sigma_k} \right) \frac{\partial k}{\partial x_j} \right]
\end{equation}

\begin{equation}
\frac{\partial \rho \varepsilon}{\partial t} +
\frac{\partial (\rho u_j \varepsilon)}{\partial x_j} = 
\frac{C_{\varepsilon 1} P - C_{\varepsilon 2} \rho \varepsilon}{T}
+ \frac{\partial}{\partial x_j} \left[
\left( \mu + \frac{\mu_t}{\sigma_{\varepsilon}} \right) \frac{\partial \varepsilon}{\partial x_j} \right]
\end{equation}

\begin{equation}
\frac{\partial \rho \zeta}{\partial t} +
\frac{\partial (\rho u_j \zeta)}{\partial x_j} = \rho f - \frac{\zeta}{k}P +
\frac{\partial}{\partial x_j} \left[
\left( \mu + \frac{\mu_t}{\sigma_{\zeta}} \right) \frac{\partial \zeta}{\partial x_j} \right]
\end{equation}

\begin{equation}
L^2\nabla^2 f - f = L^2\frac{\partial}{\partial x_j}\left(\frac{\partial f}{\partial x_j}\right) -f = 
\frac{1}{T} \left(C_1 - 1 + C_2' \frac{P}{\rho \varepsilon} \right) 
\left(\zeta - \frac{2}{3} \right)
\end{equation}

\begin{equation}
P = \tau_{ij} \frac{\partial u_i}{\partial x_j}
\end{equation}

\begin{equation}
\tau_{ij} = \mu_t \left(2S_{ij} - \frac{2}{3} \frac{\partial u_k}{\partial x_k} \delta_{ij} \right)
   - \frac{2}{3} \rho k \delta_{ij}
\end{equation}

\begin{equation}
S_{ij} = \frac{1}{2} \left( \frac{\partial u_i}{\partial x_j} + \frac{\partial u_j}{\partial x_i} \right)
\end{equation}

\begin{equation}
\mu_t = \rho C_{\mu} \zeta k T
\end{equation}

\begin{equation}
P = \mu_t S^2
\end{equation}

\begin{equation}
S=\sqrt{2 S_{ij} S_{ij}}
\end{equation}

\begin{equation}
T = {\rm max} \left[ {\rm min} \left(
\frac{k}{\varepsilon}, \frac{0.6}{\sqrt{6} C_{\mu} |S| \zeta} \right),
C_T \left( \frac{\nu}{\varepsilon} \right)^{1/2} \right]
\end{equation}

\begin{equation}
L = C_L {\rm max} \left[ {\rm min} \left(
\frac{k^{3/2}}{\varepsilon},
\frac{k^{1/2}}{\sqrt{6} C_{\mu} |S| \zeta} \right),
C_{\eta} \left( \frac{\nu^3}{\varepsilon} \right)^{1/4} \right]
\end{equation}

\begin{equation}
C_{\mu} = 0.22
\end{equation}

\begin{equation}
\sigma_k = 1.0
\end{equation}

\begin{equation}
\sigma_{\varepsilon} = 1.3
\end{equation}

\begin{equation}
\sigma_{\zeta} = 1.2
\end{equation}

\begin{equation}
C_{\varepsilon 1} = 1.4[1+(0.012/\zeta)]
\end{equation}

\begin{equation}
C_{\varepsilon 2} = 1.9
\end{equation}

\begin{equation}
C_1 = 1.4
\end{equation}

\begin{equation}
C_2' = 0.65
\end{equation}

\begin{equation}
C_T = 6
\end{equation}

\begin{equation}
C_L = 0.36
\end{equation}

\begin{equation}
C_{\eta} = 85
\end{equation}

\begin{equation}
k_w = 0
\end{equation}

\begin{equation}
\varepsilon_w = \lim_{d\to0}{\frac{2 \nu k}{d^2}}
\end{equation}

\begin{equation}
\zeta_w = 0
\end{equation}

\begin{equation}
f_w = \lim_{d\to0}{\frac{-2 \nu \zeta}{d^2}}
\end{equation}

\begin{equation}
\zeta = v^2 / k
\end{equation}

\begin{equation}
\varepsilon
\end{equation}

\begin{equation}
\varepsilon_w = 2 \nu \left( \frac{\partial k^{1/2}}{\partial \eta} \right)^2 |_w
\end{equation}

\begin{equation}
\eta
\end{equation}

\begin{equation}
\tilde \varepsilon_w = 0
\end{equation}

\begin{equation}
\tilde f_w = 0
\end{equation}

\begin{equation}
\tilde \varepsilon = \varepsilon - \frac{2 \nu k}{d^2}
\end{equation}

\begin{equation}
\tilde f = f + \frac{2 \nu \zeta}{d^2}
\end{equation}

\begin{equation}
\varepsilon_w = \frac{2 \nu_1 k_1}{d_1^2}
\end{equation}

\begin{equation}
f_w = -\frac{2 \nu_1 \zeta_1}{d_1^2}
\end{equation}

\begin{equation}
B=1
\end{equation}

\end{document}
