\begin{document}

\begin{equation}
\overline \rho R'_{ij}
\end{equation}

\begin{equation}
\tau_{ij}
\end{equation}

\begin{equation}
\overline \rho R'_{ij} = \tau_{ij} = -\overline {\rho u_i'' u_j''}
\end{equation}

\begin{equation}
\frac{\partial \overline \rho R'_{ij}}{\partial t} +
\frac{\partial (\overline \rho \hat u_k R'_{ij})}{\partial x_k} = -\overline \rho P_{ij} -
\overline \rho \Pi_{ij} + \frac{2}{3} \beta^* \overline \rho \omega k \delta_{ij} +
\frac{\partial}{\partial x_k} \left[ \left( \overline \mu + \sigma^* \mu_t \right)
\frac{\partial R'_{ij}}{\partial x_k} \right]
\end{equation}

\begin{equation}
\frac{\partial (\overline \rho \omega)}{\partial t} +
  \frac{\partial (\overline \rho \hat u_k \omega)}{\partial x_k}
  = \frac{\alpha \overline \rho \omega}{k} R'_{ij} \frac{\partial \hat u_i}{\partial x_j} -
  \beta \overline \rho \omega^2 + \frac{\partial}{\partial x_k}
  \left[ \left( \overline \mu + \sigma \mu_t \right)
  \frac{\partial \omega}{\partial x_k} \right] +
  \sigma_d \frac{\overline \rho}{\omega} \frac{\partial k}{\partial x_j}
  \frac{\partial \omega}{\partial x_j}
\end{equation}

\begin{equation}
P_{ij} = R'_{ik}
\frac{\partial \hat u_j}{\partial x_k}
+ R'_{jk} \frac{\partial \hat u_i}{\partial x_k}
\end{equation}

\begin{equation}
k=-R'_{ii}/2
\end{equation}

\begin{equation}
\mu_t = \overline \rho k / \omega
\end{equation}

\begin{equation}
\Pi_{ij} = \beta^* C_1 \omega \left( R'_{ij} +
  \frac{2}{3} k \delta_{ij} \right)
  - \hat \alpha \left( P_{ij} - \frac{2}{3} P \delta_{ij} \right)
  - \hat \beta \left( D_{ij} - \frac{2}{3} P \delta_{ij} \right)
  - \hat \gamma k \left( S_{ij} - \frac{1}{3} S_{kk} \delta_{ij} \right)
\end{equation}

\begin{equation}
D_{ij} = R'_{ik}
\frac{\partial \hat u_k}{\partial x_j}
+ R'_{jk} \frac{\partial \hat u_k}{\partial x_i}
\end{equation}

\begin{equation}
P = P_{kk}/2
\end{equation}

\begin{equation}
\hat \alpha = (8+C_2)/11
\end{equation}

\begin{equation}
\hat \beta = (8 C_2-2)/11
\end{equation}

\begin{equation}
\hat \gamma = (60 C_2 - 4)/55
\end{equation}

\begin{equation}
C_1 = 9/5
\end{equation}

\begin{equation}
C_2 = 10/19
\end{equation}

\begin{equation}
\alpha = 13/25
\end{equation}

\begin{equation}
\beta = \beta_0 f_{\beta}
\end{equation}

\begin{equation}
\beta^* = 9/100
\end{equation}

\begin{equation}
\sigma=0.5
\end{equation}

\begin{equation}
\sigma^*=0.6
\end{equation}

\begin{equation}
\beta_0 = 0.0708
\end{equation}

\begin{equation}
\hat S_{ki} = S_{ki} - \frac{1}{2} \frac{\partial \hat u_m}{\partial x_m} \delta_{ki}
\end{equation}

\begin{equation}
\omega
\end{equation}

\begin{equation}
R'_{ij, wall} = 0
\end{equation}

\begin{equation}
S_{ij} = \frac{1}{2} \left( \frac{\partial \hat u_i}{\partial x_j} +
\frac{\partial \hat u_j}{\partial x_i} \right)
\end{equation}

\begin{equation}
W_{ij} = \frac{1}{2} \left( \frac{\partial \hat u_i}{\partial x_j} -
\frac{\partial \hat u_j}{\partial x_i} \right)
\end{equation}

\begin{equation}
\Pi_{ij} = - C_1 \varepsilon a_{ij} +
(\hat \alpha + \hat \beta) k \left( a_{ik} S_{jk} +
a_{jk} S_{ik} - \frac{2}{3} a_{kl} S_{kl} \delta_{ij} \right) +
(\hat \alpha - \hat \beta) k \left(a_{ik} W_{jk} + a_{jk} W_{ik} \right) +
\left[ \frac{4}{3} \left( \hat \alpha + \hat \beta \right) - \hat \gamma \right]
k \left( S_{ij} - \frac{1}{3}S_{kk} \delta_{ij} \right)
\end{equation}

\begin{equation}
a_{ij} = -\frac{R'_{ij}}{k} - \frac{2}{3}\delta_{ij}
\end{equation}

\begin{equation}
\varepsilon = \beta^* k \omega
\end{equation}

\begin{equation}
\chi_{\omega} = \left| \frac{W_{ij} W_{jk} \hat S_{ki}}
  {(\beta^* \omega)^3} \right|
\end{equation}

\begin{equation}
B=1
\end{equation}

\end{document}
