\begin{document}

\begin{equation}
\frac{\partial R}{\partial t} + \frac{\partial u_j R}{\partial x_j}
= \frac{\partial}{\partial x_j} \left[(\sigma_R R + \nu) \frac{\partial R}{\partial x_j} \right]
+C_1RS + f_1 C_{2k\omega} \frac{R}{S} \frac{\partial R}{\partial x_j} \frac{\partial S}{\partial x_j}
-(1-f_1)C_{2k\epsilon}R^2 \left(\frac{\frac{\partial S}{\partial x_j} \frac{\partial S}{\partial x_j}}{S^2} \right)
\end{equation}

\begin{equation}
\mu_t = \rho f_{\mu} R
\end{equation}

\begin{equation}
S=\sqrt{2 S_{ij} S_{ij} }
\end{equation}

\begin{equation}
S_{ij} = \frac{1}{2} \left( \frac{\partial u_i}{\partial x_j} +
\frac{\partial u_j}{\partial x_i} \right)
\end{equation}

\begin{equation}
f_{\mu} = \frac{\chi^3}{\chi^3 + C_w^3}
\end{equation}

\begin{equation}
\chi = R/ \nu
\end{equation}

\begin{equation}
\nu = \mu/ \rho
\end{equation}

\begin{equation}
f_1 = \rm{min} \left(\rm{tanh} \left(arg_1^4 \right), 0.9 \right)
\end{equation}

\begin{equation}
arg_1 = \frac{1+ \frac{d \sqrt{RS}}{\nu}}{1+
\left[ \frac{\rm{max}(d \sqrt{RS}, 1.5 R)}{20 \nu} \right]^2}
\end{equation}

\begin{equation}
C_{1k\omega}=0.0829
\end{equation}

\begin{equation}
C_{1k\epsilon}=0.1127
\end{equation}

\begin{equation}
C_1 = f_1(C_{1k\omega} - C_{1k\epsilon}) + C_{1k\epsilon}
\end{equation}

\begin{equation}
\sigma_{k \omega} = 0.72
\end{equation}

\begin{equation}
\sigma_{k \epsilon} = 1.0
\end{equation}

\begin{equation}
\sigma_R = f_1(\sigma_{k \omega} - \sigma_{k \epsilon}) + \sigma_{k \epsilon}
\end{equation}

\begin{equation}
C_{2k\omega} = \frac{C_{1k\omega}}{\kappa^2} + \sigma_{k \omega}
\end{equation}

\begin{equation}
C_{2k\epsilon} = \frac{C_{1k\epsilon}}{\kappa^2} + \sigma_{k \epsilon}
\end{equation}

\begin{equation}
\kappa = 0.41
\end{equation}

\begin{equation}
C_w = 8.54
\end{equation}

\begin{equation}
R_{wall} = 0
\end{equation}

\begin{equation}
R_{farfield} = 3 \nu_{\infty} : to : 5 \nu_{\infty}
\end{equation}

\begin{equation}
\rho
\end{equation}

\begin{equation}
S = {\rm max}(S,10^{-16} s^{-1})
\end{equation}

\begin{equation}
B=1
\end{equation}

\end{document}
