\begin{document}

\begin{equation}
\frac{\partial (\rho k)}{\partial t} + \frac{\partial (\rho u_j k)}{\partial x_j}
  = \cal P - \rho \varepsilon  + \frac{\partial}{\partial x_j}
  \left[\left(\mu + \frac{\mu_t}{\sigma_k} \right)\frac{\partial k}{\partial x_j}\right]
\end{equation}

\begin{equation}
\frac{\partial (\rho \varepsilon)}{\partial t} + 
  \frac{\partial (\rho u_j \varepsilon)}{\partial x_j}
  = \frac{1}{T_t} \left( C_{\varepsilon 1} \cal P -
  C_{\varepsilon 2} \rho \varepsilon + 
  C_{\varepsilon 3} E \right) + \frac{\partial}{\partial x_j}
  \left[ \left( \mu + \frac{\mu_t}{\sigma_{\varepsilon}} \right)
  \frac{\partial \varepsilon}{\partial x_j} \right]
\end{equation}

\begin{equation}
\frac{\partial (\rho R_t)}{\partial t} +  \frac{\partial (\rho u_j R_t)}{\partial x_j}
  = \left( C_1 - C_2f_2 \right) \sqrt{\rho R_t \cal P}
  -\rho C_3 D + \frac{\partial}{\partial x_j}
  \left[ \left( \mu + \frac{\mu_t}{\sigma_{Rt}} \right)
  \frac{\partial R_t}{\partial x_j} \right]
\end{equation}

\begin{equation}
P = \tau_{ij} \frac{\partial u_i}{\partial x_j}
\end{equation}

\begin{equation}
\tau_{ij} = \mu_t \left(2S_{ij} - \frac{2}{3} \frac{\partial u_k}{\partial x_k} \delta_{ij} \right)
   - \frac{2}{3} \rho k \delta_{ij}
\end{equation}

\begin{equation}
S_{ij} = \frac{1}{2} \left( \frac{\partial u_i}{\partial x_j} + \frac{\partial u_j}{\partial x_i} \right)
\end{equation}

\begin{equation}
\varepsilon
\end{equation}

\begin{equation}
E = \rho \sqrt{\varepsilon T_t} {\rm max}\left( \sqrt{k}, (\nu \varepsilon)^{1/4} \right)
   {\rm max} \left( \frac{\partial k}{\partial x_j} 
   \frac{\partial \tau}{\partial x_j},0 \right)
\end{equation}

\begin{equation}
\tau = \frac{k}{\varepsilon}
\end{equation}

\begin{equation}
T_t = \tau \left[ {\rm max} \left( 1, \sqrt{\frac{2}{Re_t}} \right) \right]
\end{equation}

\begin{equation}
Re_t = \frac{k \tau}{\nu}
\end{equation}

\begin{equation}
f_2 = \frac{{\rm tanh}\sqrt{\chi}}{{\rm tanh}\left(\sqrt{2} C_{\mu}^{1/4} \chi\right)}
\end{equation}

\begin{equation}
\chi = \frac{R_t}{C_{\mu} \nu}
\end{equation}

\begin{equation}
f_2 = 1
\end{equation}

\begin{equation}
  D = \left\{
  \begin{array}{l l}
  \left(\partial R_t / \partial x_j\right)
  \left(\partial R_t / \partial x_j\right), & \lambda>0 \\
  0, & \lambda \leq 0
  \end{array}\right.
\end{equation}

\begin{equation}
\lambda = \frac{\partial Q}{\partial x_j} \frac{\partial R_t}{\partial x_j}
\end{equation}

\begin{equation}
Q = \sqrt{(U-U_0)^2 + (V-V_0)^2 + (W-W_0)^2}
\end{equation}

\begin{equation}
f_{\mu,k-\varepsilon} = \frac{1-{\rm exp}(-A_{\mu}Re_t)}{1-{\rm exp}(-\sqrt{Re_t})}
{\rm max}\left( 1, \sqrt{2/Re_t} \right)
\end{equation}

\begin{equation}
f_{\mu,Rt} = \frac{{\rm tanh}(\alpha \chi^2)}
{{\rm tanh}(\beta \chi^2)}
\end{equation}

\begin{equation}
\mu_{t,k-\varepsilon} = {\rm min} \left( C_{\mu} f_{\mu,k-\varepsilon} \rho k \tau,
  \frac{\phi \rho k}{|S|} \right)
\end{equation}

\begin{equation}
\mu_{t,Rt} = f_{\mu,Rt} \rho R_t
\end{equation}

\begin{equation}
\mu_t = {\rm max} \left( \mu_{t,k-\varepsilon},\mu_{t,Rt} \right)
\end{equation}

\begin{equation}
{\rm abs}(S) = |S|
\end{equation}

\begin{equation}
\phi
\end{equation}

\begin{equation}
\phi = 2/3
\end{equation}

\begin{equation}
\phi = 0.31
\end{equation}

\begin{equation}
\sigma_k = 1.0
\end{equation}

\begin{equation}
\sigma_{\varepsilon} = 1.3
\end{equation}

\begin{equation}
\sigma_{Rt} = 1.0
\end{equation}

\begin{equation}
C_{\varepsilon 1} = 1.44
\end{equation}

\begin{equation}
C_{\varepsilon 2} = 1.92
\end{equation}

\begin{equation}
C_{\varepsilon 3} = 0.3
\end{equation}

\begin{equation}
A_{\mu} = 0.007
\end{equation}

\begin{equation}
\alpha = 0.00015
\end{equation}

\begin{equation}
\beta = 0.2
\end{equation}

\begin{equation}
C_1 = C_2 + \kappa^2(C_3 - 1/\sigma_{Rt}) = 39.918
\end{equation}

\begin{equation}
C_2 = (12/11) \sqrt{\beta/\alpha} = 39.834
\end{equation}

\begin{equation}
C_3 = 3/(2 \sigma_{Rt}) = 1.5
\end{equation}

\begin{equation}
k
\end{equation}

\begin{equation}
R_t
\end{equation}

\begin{equation}
k_w = 0
\end{equation}

\begin{equation}
R_{t,w} = 0
\end{equation}

\begin{equation}
\varepsilon_w = 2 \nu \left(\frac{\partial \sqrt{k}}{\partial n} \right)_w^2
\end{equation}

\begin{equation}
Re_t
\end{equation}

\begin{equation}
B=1
\end{equation}

\end{document}
