\begin{document}

\begin{equation}
\tau _{ij}^{(ARSM)} =  - \rho k\left( {{\beta _1}\;{T_{ij}^{(1)}} + {\beta _2}\;{T_{ij}^{(2)}} + 
{\beta _4}\;{T_{ij}^{(4)}} + \frac{2}{3}{\delta _{ij}}} \right)
\end{equation}

\begin{equation}
{T_{ij}^{(1)}} = \left[ {{S_{ij}^*} - \frac{1}{3}tr\left\{ {{S^*}} \right\}} \right]
\end{equation}

\begin{equation}
{T_{ij}^{(2)}} = \left[ {{S_{ik}^*S_{kj}^*} - \frac{1}{3}tr\left\{ {{S^{*2}}} \right\}} \right]
\end{equation}

\begin{equation}
{T_{ij}^{(4)}} = \left[ {{S_{ik}^*}{W_{kj}^*} - {W_{ik}^*}{S_{kj}^*}} \right]
\end{equation}

\begin{equation}
{S_{ij}^*} = \tau S_{ij}
\end{equation}
 
\begin{equation}
{W_{ij}^*} = \tau W_{ij}
\end{equation}

\begin{equation}
{S_{ij}} = \frac{1}{2} \left( \frac{\partial u_i}{\partial x_j} 
             + \frac{\partial u_j}{\partial x_i}\right)
\end{equation}
 
\begin{equation}
{W_{ij}} = \frac{1}{2} \left( \frac{\partial u_i}{\partial x_j} 
             - \frac{\partial u_j}{\partial x_i}\right)
\end{equation}

\begin{equation}
\tau  = \frac{{C_\mu ^{1/4}}}{{{C_\mu }}}\frac{{(kL)}}{{{k^{3/2}}}}
\end{equation}
 
\begin{equation}
\frac{{\partial \rho k}}{{\partial t}} + \frac{{\partial \rho {u_j}k}}{{\partial {x_j}}} 
   = {{P_k} + \frac{\partial }{{\partial {x_j}}}\left( {\left( {{\mu} + 
   {\sigma _{k}}{\mu _t}} \right)\frac{{\partial \rho k}}{{\partial {x_j}}}} \right)  - 
   C_w{\mu}\frac{k}{{{d^2}}}} - {C_{k}}\rho \frac{{{k^{2.5}}}}{{(kL)}}
\end{equation}

\begin{equation}
\frac{{\partial \rho (kL)}}{{\partial t}} + \frac{{\partial \rho {u_j}(kL)}}{{\partial {x_j}}} 
   = {{C_{{(kL)}_{\scriptstyle 1}}}\frac{{(kL)}}{k}{P_{kL}} + 
   \frac{\partial }{{\partial {x_j}}}\left( {\left( {{\mu} + 
   {\sigma _{(kL)}}{\mu _t}} \right)\frac{{\partial \rho (kL)}}{{\partial {x_j}}}} \right) - 
   6{\mu}\frac{{(kL)}}{{{d^2}}}{f_{(kL)}}}
   - {C_{{(kL)}_{\scriptstyle 2}}}\rho {k^{1.5}}
\end{equation}
 
\begin{equation}
P_k = \tau_{ij} \frac{\partial u_i}{\partial x_j}
\end{equation}

\begin{equation}
P_{kL} = \max ({P_k},{\mu _t}^{(L)}{S^2})
\end{equation}

\begin{equation}
{\mu _t} = \frac{{C_\mu ^*}}{{{C_\mu }}}C_\mu ^{1/4}\frac{{\rho (kL)}}{{{k^{1/2}}}}
\end{equation}

\begin{equation}
\rho
\end{equation}

\begin{equation}
\mu_l
\end{equation}

\begin{equation}
C_{\mu}^* \equiv -\alpha
\end{equation}

\begin{equation}
\alpha^3 + p \alpha^2 + q \alpha + r = 0
\end{equation}

\begin{equation}
k_{farfield} = 9 \times 10^{-9} {a_{ref}^2}
\end{equation}

\begin{equation}
(kL)_{farfield} = 1.5589 \times 10^{-6} \frac{\mu_{ref} a_{ref}}{\rho_{ref}}
\end{equation}

\begin{equation}
\rho_{ref}
\end{equation}

\begin{equation}
a_{ref}
\end{equation}

\begin{equation}
\mu_{ref}
\end{equation}

\begin{equation}
k_{wall} = (kL)_{wall} = 0
\end{equation}

\begin{equation}
\sigma_{(kL)} = 1.0
\end{equation}

\begin{equation}
C_{(kL)_1} = \left[ \zeta_1 - \zeta_2 \left( \frac{(kL)}{k L_{vk}} \right)^2 \right]
\end{equation}

\begin{equation}
C_{(kL)_2} = \zeta_3
\end{equation}

\begin{equation}
f_{(kL)} = \frac{1+C_{d1} \xi}{1 + \xi^4}
\end{equation}

\begin{equation}
C_{w} = 1.5
\end{equation}

\begin{equation}
C_4 = 0.6
\end{equation}

\begin{equation}
f_p=min\left[ max\left(\frac{\cal P_k}{\left(C_{\mu}^{3/4} \rho k^{5/2}/(kL) \right)}
 , C_{13} \right) , 1.0 \right]
\end{equation}

\begin{equation}
C_{13} = 0.25
\end{equation}

\begin{equation}
\beta_1 = -2 C_{\mu}^* = 2 \alpha
\end{equation}

\begin{equation}
\beta_2 = -2 a_4 a_3 \beta_1
\end{equation}

\begin{equation}
\beta_4 = a_4 a_2 \beta_1
\end{equation}

\begin{equation}
\beta_2=\beta_4=0
\end{equation}

\begin{equation}
\sigma_k = f_2 \sigma_{k1} + (1-f_2) \sigma_{k2}
\end{equation}

\begin{equation}
\sigma_{k1} = 1.0
\end{equation}

\begin{equation}
\sigma_{k2} = 0.5
\end{equation}

\begin{equation}
f_2 = tanh \left(\Gamma^2\right)
\end{equation}

\begin{equation}
\Gamma = max\left(2 \frac{\sqrt{k}}{C_\mu \omega d}, \frac{500 \nu}{d^2 \omega}\right)
\end{equation}

\begin{equation}
\omega = \frac{k^{3/2}}{(kL) C_\mu^{1/4}}
\end{equation}

\begin{equation}
\tau _{ij} = f_2 \tau _{ij}^{(ARSM)} + (1-f_2) \tau _{ij}^{(L)}
\end{equation}

\begin{equation}
\tau _{ij}^{(L)}
\end{equation}

\begin{equation}
C_k = C_{\mu}^{3/4} (1+f_c)
\end{equation}

\begin{equation}
C_{(kL)_2} = \zeta_3 + 2.5 C_{\mu}^{3/4} f_c
\end{equation}

\begin{equation}
f_c = 1.5 (1.0-f_2)\left( M_t^2 - M_0^2 \right) \icalH \left[ M_t^2 - M_0^2 \right]
\end{equation}

\begin{equation}
M_t = \sqrt{\frac{2 k}{a^2}}
\end{equation}

\begin{equation}
M_0=0.19
\end{equation}

\begin{equation}
{\mu _t}^{(L)} = C_\mu ^{1/4}\frac{{\rho (kL)}}{{{k^{1/2}}}}
\end{equation}

\begin{equation}
a_4 = \left[ \gamma_1^* - 2 \gamma_0^* \left( -C_{\mu}^* \right) \eta^2 \tau^2 \right]^{-1}
\end{equation}


\begin{equation}
B=1
\end{equation}

\end{document}
